Splinter/Paged/JournalIfc.i.dfy
@@ -36,7 +36,7 @@ abstract module JournalIfc {
     ensures IEJ(out) == IPJ(pj)
 
   // TODO rename PJournalSeqEnd, I guess
-  function JournalSeqEnd(pj: PersistentJournal) : (out:Option<LSN>)
+  function PJournalSeqEnd(pj: PersistentJournal) : (out:Option<LSN>)
     requires PWF(pj)
     ensures out.Some? == IPJ(pj).MsgHistory?
     ensures out.Some? ==> out.value == IPJ(pj).seqEnd
@@ -49,27 +49,27 @@ abstract module JournalIfc {
   predicate JournalIncludesSubseq(ej: EphemeralJournal, msgs: MsgHistory)
     requires EWF(ej)
     requires msgs.WF()
-    ensures JournalIncludesSubseq(ej, msgs) <==> IEJ(ej).IncludesSubseq(msgs)
+    ensures JournalIncludesSubseq(ej, msgs) ==> IEJ(ej).IncludesSubseq(msgs)
 
   function JournalConcat(ej: EphemeralJournal, msgs: MsgHistory) : (out:EphemeralJournal)
     requires EWF(ej)
     requires msgs.WF()
     requires msgs.EmptyHistory? || EJournalSeqEnd(ej).None? || msgs.CanFollow(EJournalSeqEnd(ej).value)
-    ensures EWF(JournalConcat(ej, msgs))
     ensures EWF(out)
     ensures IEJ(ej).Concat(msgs) == IEJ(out)
 
   predicate JournalCanFreeze(ej: EphemeralJournal, startLsn: LSN, endLsn: LSN)
     requires EWF(ej)
-    ensures JournalCanFreeze(ej, startLsn, endLsn) <==>
-      (IEJ(ej).CanDiscardTo(startLsn) && IEJ(ej).CanDiscardTo(endLsn))
+    ensures JournalCanFreeze(ej, startLsn, endLsn) ==>
+      (startLsn == endLsn ||
+       (IEJ(ej).CanDiscardTo(startLsn) && IEJ(ej).CanDiscardTo(endLsn)))
 
   function JournalFreeze(ej: EphemeralJournal, startLsn: LSN, endLsn: LSN) : (out:PersistentJournal)
     requires EWF(ej)
     requires JournalCanFreeze(ej, startLsn, endLsn)
     requires startLsn <= endLsn
     ensures PWF(out)
-    ensures IPJ(out) == IEJ(ej).DiscardOld(startLsn).DiscardRecent(endLsn)
+    ensures IPJ(out) == if startLsn==endLsn then EmptyHistory else IEJ(ej).DiscardOld(startLsn).DiscardRecent(endLsn)
 
   predicate CanDiscardOld(ej: EphemeralJournal, lsn: LSN)
     requires EWF(ej)
