Splinter/Paged/Bundle.i.dfy
@@ -1,5 +1,10 @@
 include "AbstractJournal.i.dfy"
+include "PagedJournal.i.dfy"
 
 // Hey look, this abstract journal satisfies the refinement.
 module AbstractJournalRefinement refines PagedSystemRefinement(AbstractJournal) {
+}
+
+// Ooh, and so does this Paged journal
+module PagedJournalRefinement refines PagedSystemRefinement(PagedJournal) {
 }
