Splinter/Paged/PagedJournal.i.dfy
@@ -1,0 +1,615 @@
+include "JournalIfc.i.dfy"
+
+module PagedJournal refines JournalIfc {
+  import opened Sequences
+
+  // This module constructs a journal out of a chain of page-sized journal records.
+  // It satisfyies JournalIfc, so it can enjoy the PagedSystemRefinement result.
+
+  datatype JournalRecord = JournalRecord(
+    messageSeq: MsgHistory,
+    priorRec: Option<JournalRecord>
+  )
+  {
+    predicate WF()
+    {
+      && messageSeq.WF()
+
+      // Disallow empty records. Means we can always talk about seqEnd
+      && messageSeq.MsgHistory?
+    }
+  }
+
+  // Does a JournalRecord begin a sensible linked list?
+
+  datatype ReceiptLine = ReceiptLine(
+    journalRec: JournalRecord,
+    // None means the JournalRecord was malformed, at least with respect to the
+    // boundaryLSN.
+    interpretation: Option<MsgHistory>)
+  {
+    predicate WF() {
+      && journalRec.WF()
+      && (interpretation.Some? ==> interpretation.value.WF())
+    }
+
+    function Truncated(boundaryLSN: LSN) : MsgHistory
+      requires WF()
+    {
+      if journalRec.messageSeq.CanDiscardTo(boundaryLSN)
+      then journalRec.messageSeq.DiscardOld(boundaryLSN)
+      else journalRec.messageSeq
+    }
+  }
+
+  datatype Receipt = Receipt(boundaryLSN: LSN, lines: seq<ReceiptLine>)
+  {
+    predicate LineRespectsLinkedList(i: nat)
+      requires 0<i<|lines|
+    {
+      lines[i].journalRec.priorRec == Some(lines[i-1].journalRec)
+    }
+
+    predicate LinesRespectLinkedList()
+    {
+      forall i | 0<i<|lines| :: LineRespectsLinkedList(i)
+    }
+
+    predicate FirstLineTJValid()
+    {
+      // The first record is well-formed, is a history, and includes the boundaryLSN.
+      0<|lines| ==> (
+        && var jr := lines[0].journalRec;
+        && jr.WF()
+        && jr.messageSeq.MsgHistory?
+        && jr.messageSeq.seqStart <= boundaryLSN < jr.messageSeq.seqEnd
+      )
+    }
+
+    // A valid receipt either shows a valid TJ, or shows that the TJ starts in
+    // an invalid way.
+    predicate FirstLineValid()
+    {
+      0<|lines| ==> (
+        // the journalRec is borked (so !TJValid())
+        || !lines[0].journalRec.WF()
+        // or the first record somehow goes too far into the past (presumably
+        // because that's the only record; otherwise stitching would fail first
+        // in BuildReceipt).
+        || (
+          && lines[0].journalRec.messageSeq.MsgHistory?
+          && lines[0].journalRec.messageSeq.seqEnd <= boundaryLSN
+          )
+        // or if we're at the end of the linked list (but perhaps didn't reach the boundaryLSN)
+        || lines[0].journalRec.priorRec.None?
+        // Or it's actually valid -- it provides boundaryLSN.
+        || FirstLineTJValid()
+      )
+    }
+
+    predicate InterpretationWF(i: nat)
+      requires i<|lines|
+    {
+      lines[i].interpretation.Some? ==> lines[i].interpretation.value.WF()
+    }
+
+    predicate InterpretationsWF()
+    {
+      forall i | 0<=i<|lines| :: InterpretationWF(i)
+    }
+
+    function LinkedInterpretation(i: nat) : Option<MsgHistory>
+      requires InterpretationsWF()
+      requires i<|lines|
+    {
+      if !lines[i].WF()
+      then None // Bogus line
+      else if i==0
+      then (
+        if !FirstLineTJValid() then None else Some(lines[i].Truncated(boundaryLSN))
+      )
+      else if lines[i-1].interpretation.None?
+      then None // previous line already bogus
+      else if
+        assert InterpretationWF(i-1); // trigger
+        !lines[i-1].interpretation.value.CanConcat(lines[i].journalRec.messageSeq)
+      then None // adjacent lines don't stitch
+      else Some(lines[i-1].interpretation.value.Concat(lines[i].journalRec.messageSeq))
+    }
+
+    predicate OneLinkedInterpretation(i: nat)
+      requires InterpretationsWF()
+      requires i<|lines|
+    {
+      lines[i].interpretation == LinkedInterpretation(i)
+    }
+
+    predicate {:opaque} LinkedInterpretations() // TODO(jonh): can probably remove opaque now?
+      requires InterpretationsWF()
+    {
+      forall i | 0<=i<|lines| :: OneLinkedInterpretation(i)
+    }
+
+    // Valid means this receipt correctly explains the fate of the
+    // TruncatedJournal it represents, whether that be its interpretation
+    // or the fact that it's uninterpretable.
+    predicate Valid()
+    {
+      && LinesRespectLinkedList()
+      && FirstLineValid()
+      && InterpretationsWF()
+      && LinkedInterpretations()
+    }
+
+    // TJValid means the TruncatedJournal this receipt represents is itself
+    // valid -- it has a valid interpretation.
+    predicate TJValid()
+      requires Valid()
+    {
+      // Final interpretation is happy.
+      && (0 < |lines| ==> && Last(lines).interpretation.Some?)
+    }
+
+    lemma SomeInterpretation(j: nat)
+      requires Valid()
+      requires TJValid()
+      requires j <= |lines|
+      ensures forall i | j <= i < |lines| :: lines[i].interpretation.Some?
+      decreases |lines|-j
+    {
+      forall i | j <= i < |lines| ensures lines[i].interpretation.Some? {
+        if i < |lines|-1 {
+          SomeInterpretation(i + 1);  // i+1 is some by induction hypothesis
+          assert OneLinkedInterpretation(i+1) by { // if i were None, contradiction!
+            reveal_LinkedInterpretations();
+          }
+        }
+      }
+    }
+
+    lemma JournalRecsAllWF()
+      requires Valid()
+      requires TJValid()
+      ensures forall i | 0<=i<|lines| :: lines[i].journalRec.WF()
+    {
+      SomeInterpretation(0);
+      forall i | 0<=i<|lines| ensures lines[i].journalRec.WF() {
+        assert InterpretationWF(i); // trigger
+        assert OneLinkedInterpretation(i) by { reveal_LinkedInterpretations(); }
+      }
+    }
+
+    // A package of popular facts about TJValid receipts.
+    lemma TJFacts()
+      requires Valid()
+      requires TJValid()
+      ensures forall i | 0<=i<|lines| :: lines[i].interpretation.Some?
+      ensures forall i | 0<=i<|lines| :: lines[i].journalRec.WF()
+      ensures FirstLineTJValid()
+    {
+      SomeInterpretation(0);
+      JournalRecsAllWF();
+      if 0 < |lines| {
+        assert OneLinkedInterpretation(0) by { reveal_LinkedInterpretations(); }
+      }
+    }
+
+    function I() : MsgHistory
+      requires Valid()
+      requires TJValid()
+    {
+      if |lines|==0
+      then EmptyHistory
+      else Last(lines).interpretation.value
+    }
+
+    // Returns the message history represented by journal page i in this receipt
+    function MessageSeqAt(i: nat) : (out:MsgHistory)
+      requires i < |lines|
+      requires Valid()
+      requires TJValid()  // maybe?
+      ensures out.WF()
+    {
+      var rec := lines[i].journalRec;
+      JournalRecsAllWF();
+      if rec.messageSeq.CanDiscardTo(boundaryLSN)
+      then rec.messageSeq.DiscardOld(boundaryLSN)
+      else rec.messageSeq
+    }
+  }
+
+  // Constructive evidence that a Valid receipt exists for each TJ
+  function BuildReceipt(boundaryLSN: LSN, optRec: Option<JournalRecord>) : (out:Receipt)
+    ensures out.Valid()
+  {
+    // A global Receipt(0,[]).reveal_LinkedInterpretations() makes this function
+    // prove, but because this function's body is reachable from WF, pollutes
+    // lots of later CheckWellformeds to run out of resource.
+    if optRec.None?
+    then var out := Receipt(boundaryLSN, []);
+      assert out.Valid() by { Receipt(0,[]).reveal_LinkedInterpretations(); }
+      out
+    else
+      var rec := optRec.value;
+      if !rec.WF()
+      then
+        // Malformed record
+        var out := Receipt(boundaryLSN, [ReceiptLine(rec, None)]);
+        assert out.Valid() by { Receipt(0,[]).reveal_LinkedInterpretations(); }
+        out
+      else if rec.messageSeq.seqEnd <= boundaryLSN
+      then
+        // Uh, this journal record ends before boundaryLSN? Why do we have it?
+        var out := Receipt(boundaryLSN, [ReceiptLine(rec, None)]);
+        assert out.Valid() by { Receipt(0,[]).reveal_LinkedInterpretations(); }
+        out
+      else if rec.messageSeq.seqStart <= boundaryLSN
+      then
+        // boundaryLSN satisfied here; can stop decoding. Don't care what lies
+        // beyond!
+        var out := Receipt(boundaryLSN, [ReceiptLine(rec, Some(rec.messageSeq.DiscardOld(boundaryLSN)))]);
+        assert out.Valid() by { Receipt(0,[]).reveal_LinkedInterpretations(); }
+        out
+      else if rec.priorRec.None?
+      then (
+        assert boundaryLSN < rec.messageSeq.seqStart;
+        // Uh oh, we needed a prior rec!
+        var out := Receipt(boundaryLSN, [ReceiptLine(rec, None)]);
+        assert out.Valid() by { Receipt(0,[]).reveal_LinkedInterpretations(); }
+        out
+      )
+      else
+        // Recurse.
+        var priorReceipt := BuildReceipt(boundaryLSN, rec.priorRec);
+        var priorInterpretation := Last(priorReceipt.lines).interpretation;
+        var newInterpretation :=
+          if
+            // Recursion was invalid
+            || priorInterpretation.None?
+            // Or didn't stitch.
+            || !priorInterpretation.value.CanConcat(rec.messageSeq)
+          then None
+          else Some(priorReceipt.I().Concat(rec.messageSeq));
+        var out := Receipt(boundaryLSN,
+          priorReceipt.lines + [ReceiptLine(rec, newInterpretation)]);
+        assert out.Valid() by {
+          // trigger some features of the base case lines
+          forall i | 0<=i<|out.lines| ensures out.InterpretationWF(i) {
+            if i<|out.lines|-1 {
+              assert priorReceipt.InterpretationWF(i);
+            }
+          }
+          forall i | 0<i<|out.lines| ensures out.LineRespectsLinkedList(i) {
+            if i<|out.lines|-1 {
+              assert priorReceipt.LineRespectsLinkedList(i);
+            }
+          }
+          assert out.LinkedInterpretations() by {
+            out.reveal_LinkedInterpretations();
+            forall i | 0<=i<|out.lines| ensures out.OneLinkedInterpretation(i) {
+              if i<|out.lines|-1 {
+                assert priorReceipt.OneLinkedInterpretation(i);
+              }
+            }
+          }
+        }
+        out
+  }
+
+  // A TruncatedJournal is some long chain but which we ignore beyond the boundaryLSN
+  // (because we have a map telling us that part of the history).
+  // In the refinement layer below, we'll have some situations where the disk has extra
+  // journal records, but we'll ignore them in the refinement (since we never read them)
+  // and instead supply a None? for the interpretation at this layer.
+  // That's what keeps us out of trouble when those un-read pages get reclaimed -- we don't
+  // want to have to say we can interpret them.
+  datatype TruncatedJournal = TruncatedJournal(
+    boundaryLSN : LSN,  // exclusive: lsns <= boundaryLSN are discarded
+    freshestRec: Option<JournalRecord>)
+  {
+    function prior() : TruncatedJournal
+      requires freshestRec.Some?
+    {
+      TruncatedJournal(boundaryLSN, freshestRec.value.priorRec)
+    }
+
+    function BuildReceiptTJ() : Receipt
+    {
+      BuildReceipt(boundaryLSN, freshestRec)
+    }
+
+    predicate WF() {
+      && var receipt := BuildReceiptTJ();
+      && receipt.Valid()
+      && receipt.TJValid()
+    }
+
+    predicate Empty()
+    requires WF()
+    {
+      freshestRec.None?
+    }
+
+    function SeqEnd() : LSN
+      requires WF()
+      requires !Empty()
+    {
+      freshestRec.value.messageSeq.seqEnd
+    }
+
+    function I() : MsgHistory
+      requires WF()
+    {
+      BuildReceiptTJ().I()
+    }
+
+    function DiscardOld(lsn: LSN) : (out:TruncatedJournal)
+      requires WF()
+      requires I().CanDiscardTo(lsn)
+      ensures out.WF()
+      ensures out.I() == I().DiscardOld(lsn)
+    {
+      assume false;
+      TruncatedJournal(lsn, freshestRec)
+    }
+
+    // TODO(jonh): We need an internal operation that replaces a chain
+    // with another chain with a None instead of a dereference when the
+    // links go back before boundaryLSN, to represent journal truncation.
+
+    // msgs appears as the (boundary-truncated) contents of the i'th entry in the
+    // receipt
+    predicate IncludesSubseqAt(msgs: MsgHistory, i: nat)
+      requires WF()
+      requires msgs.WF()
+    {
+      && i < |BuildReceiptTJ().lines|
+      //&& BuildReceiptTJ().MessageSeqAt(i) == msgs // TODO deleteme
+      && BuildReceiptTJ().MessageSeqAt(i).IncludesSubseq(msgs)
+    }
+
+    lemma SubseqEntireOfInterpretation(msgs: MsgHistory, i: nat)
+      requires WF()
+      requires msgs.WF()
+      requires IncludesSubseqAt(msgs, i)
+      ensures I().IncludesSubseq(msgs)
+    {
+      // Propagate subseq relation inductively down the receipt
+      var receipt := BuildReceiptTJ();
+      receipt.TJFacts();
+      var j:=i;
+      assert receipt.OneLinkedInterpretation(j) by { receipt.reveal_LinkedInterpretations(); }
+
+      while j<|receipt.lines|-1
+        invariant j<|receipt.lines|
+        invariant var jint := receipt.lines[j].interpretation;
+              && jint.Some?  && jint.value.WF() && jint.value.IncludesSubseq(msgs)
+      {
+        assert receipt.OneLinkedInterpretation(j+1) by { receipt.reveal_LinkedInterpretations(); }
+        j:=j+1;
+      }
+    }
+
+    lemma LsnBelongs(lsn: LSN)
+      requires BuildReceiptTJ().Valid()
+      requires BuildReceiptTJ().TJValid()
+      requires !Empty()
+      requires boundaryLSN <= lsn < SeqEnd()
+      ensures lsn in BuildReceiptTJ().I().LSNSet()
+      decreases freshestRec
+    {
+      if lsn < Last(BuildReceiptTJ().lines).journalRec.messageSeq.seqStart {
+        // If it's not it in the last journal record, it's gotta be in here
+        // somewhere. Look upstream.
+        prior().LsnBelongs(lsn);
+      }
+    }
+
+// TODO delete
+//    predicate InterpretationCanDiscardAt(lsn: LSN, i: nat)
+//    {
+//      && WF()
+//      && i < |BuildReceiptTJ().lines|
+//      && var interpi := BuildReceiptTJ().lines[i].interpretation;
+//      && interpi.Some?
+//      && interpi.value.CanDiscardTo(lsn)
+//    }
+//
+//    lemma InterpretationCanDiscardTo(lsn: LSN, i: nat)
+//      requires InterpretationCanDiscardAt(lsn, i)
+//      ensures I().CanDiscardTo(lsn)
+//    {
+//      // Propagate CanDiscardTo relation inductively down the receipt
+//      var receipt := BuildReceiptTJ();
+//      receipt.SomeInterpretation(0);
+//      var j:=i;
+//      assert receipt.OneLinkedInterpretation(j) by { receipt.reveal_LinkedInterpretations(); }
+//
+//      while j<|receipt.lines|-1
+//        invariant j<|receipt.lines|
+//        invariant var jint := receipt.lines[j].interpretation;
+//              && jint.Some?  && jint.value.WF() && jint.value.CanDiscardTo(lsn)
+//      {
+//        assert receipt.OneLinkedInterpretation(j+1) by { receipt.reveal_LinkedInterpretations(); }
+//        assert receipt.lines[j+1].interpretation.value.CanDiscardTo(lsn);
+//        j:=j+1;
+//      }
+//    }
+  }
+
+  type PersistentJournal = TruncatedJournal
+
+  datatype EphemeralJournal = EphemeralJournal(
+    truncatedJournal: TruncatedJournal,
+    unmarshalledTail: MsgHistory
+  )
+  {
+    predicate WF() {
+      && truncatedJournal.WF()
+      && unmarshalledTail.WF()
+      && (unmarshalledTail.MsgHistory? ==>
+          truncatedJournal.I().CanConcat(unmarshalledTail)
+         )
+    }
+
+    function I() : MsgHistory
+      requires WF()
+    {
+      truncatedJournal.I().Concat(unmarshalledTail)
+    }
+  }
+
+  predicate PWF(pj: PersistentJournal) {
+    pj.WF()
+  }
+
+  predicate EWF(ej: EphemeralJournal) {
+    ej.WF()
+  }
+
+  function IPJ(pj: PersistentJournal) : (out:MsgHistory) { pj.I() }
+
+  function IEJ(ej: EphemeralJournal) : (out:MsgHistory) { ej.I() }
+
+  function Mkfs() : (out:PersistentJournal)
+    //ensures PWF(out)
+    //ensures IPJ(out).EmptyHistory?
+  {
+    TruncatedJournal(0, None)
+  }
+
+  function LoadJournal(pj: PersistentJournal) : (out:EphemeralJournal)
+    //requires PWF(pj)
+    //ensures EWF(out)
+    //ensures IEJ(out) == IPJ(pj)
+  {
+    EphemeralJournal(pj, EmptyHistory)
+  }
+
+  function PJournalSeqEnd(pj: PersistentJournal) : Option<LSN>
+    // ensures out.Some? == IPJ(pj).MsgHistory?
+  {
+    if
+      || pj.freshestRec.None?
+      || pj.boundaryLSN == pj.freshestRec.value.messageSeq.seqEnd
+    then None
+    else Some(pj.freshestRec.value.messageSeq.seqEnd)
+  }
+
+  predicate JournalIncludesSubseq(ej: EphemeralJournal, msgs: MsgHistory)
+    //requires EWF(ej)
+    //requires msgs.WF()
+  {
+    // subseq appears in committed pages
+    var out := (exists i :: ej.truncatedJournal.IncludesSubseqAt(msgs, i));
+    assert out ==> IEJ(ej).IncludesSubseq(msgs) by {
+      if out {
+        var i :| ej.truncatedJournal.IncludesSubseqAt(msgs, i);
+        ej.truncatedJournal.SubseqEntireOfInterpretation(msgs, i);
+      }
+    }
+    out
+    // We don't bother allowing you to "find" the msgs in unmarshalledTail,
+    // since the includes operation is only relevant during recovery time,
+    // during which we don't allow the unmarshalledTail.
+    // (I mean, we COULD allow Puts during that time, but why bother?)
+  }
+
+  function EJournalSeqEnd(ej: EphemeralJournal) : Option<LSN>
+  {
+    if ej.unmarshalledTail.MsgHistory?
+    then Some(ej.unmarshalledTail.seqEnd)
+    else PJournalSeqEnd(ej.truncatedJournal)
+  }
+
+  function JournalConcat(ej: EphemeralJournal, msgs: MsgHistory) : (out:EphemeralJournal)
+    //requires EWF(ej)
+    //requires msgs.WF()
+    //requires msgs.EmptyHistory? || EJournalSeqEnd(ej).None? || msgs.CanFollow(EJournalSeqEnd(ej).value)
+    // ensures EWF(out)
+    // ensures IEJ(ej).Concat(msgs) == IEJ(out)
+  {
+    EphemeralJournal(ej.truncatedJournal, ej.unmarshalledTail.Concat(msgs))
+  }
+
+  // TODO(jonh): a rewrite function that marshalls (some of?) unmarshalledTail
+
+  predicate CanDiscardOld(ej: EphemeralJournal, lsn: LSN)
+  {
+    // TODO(jonh): ref data structures efficiently, not via the interp
+    IEJ(ej).CanDiscardTo(lsn)
+  }
+
+  function DiscardOld(ej: EphemeralJournal, lsn: LSN) : EphemeralJournal
+    // requires EWF(ej)
+    // requires CanDiscardOld(ej, lsn)
+  {
+    if ej.unmarshalledTail.MsgHistory? && ej.unmarshalledTail.seqStart <= lsn
+    then
+      EphemeralJournal(Mkfs(), ej.unmarshalledTail.DiscardOld(lsn))
+    else
+      EphemeralJournal(ej.truncatedJournal.DiscardOld(lsn), ej.unmarshalledTail)
+  }
+
+  predicate JournalCanFreezeAt(ej: EphemeralJournal, startLsn: LSN, endLsn: LSN, i: nat)
+    requires ej.WF()
+  {
+    // Can't freeze anything in unmarshalledTail yet!
+    && var tj := ej.truncatedJournal;
+    // Anything we freeze must start no later than journal is already truncated.
+    && tj.boundaryLSN <= startLsn
+    // And must end at an existing page boundary.
+    // (In lower layers, that page and those before it must also be clean on disk.)
+    && var receipt := tj.BuildReceiptTJ();
+    && i < |receipt.lines|
+    && assert receipt.lines[i].journalRec.messageSeq.MsgHistory? by { receipt.JournalRecsAllWF(); }
+    && endLsn == receipt.lines[i].journalRec.messageSeq.seqEnd
+    && startLsn <= endLsn
+  }
+
+  predicate JournalCanFreeze(ej: EphemeralJournal, startLsn: LSN, endLsn: LSN)
+  {
+    var out := startLsn==endLsn || (exists i :: JournalCanFreezeAt(ej, startLsn, endLsn, i));
+    assert out && startLsn < endLsn ==> IEJ(ej).CanDiscardTo(startLsn) && IEJ(ej).CanDiscardTo(endLsn) by {
+      if out && startLsn < endLsn {
+	      var i:nat :| JournalCanFreezeAt(ej, startLsn, endLsn, i);
+	      var tj := ej.truncatedJournal;
+
+        // endLsn-1 is in the interp, so we can discard to endLsn
+        var receipt := tj.BuildReceiptTJ();
+        receipt.TJFacts();
+        tj.SubseqEntireOfInterpretation(receipt.MessageSeqAt(i), i);
+        assert receipt.MessageSeqAt(i).Contains(endLsn-1);  // trigger
+
+        // startLsn is in the interp, so we can discard to it
+	      tj.LsnBelongs(startLsn);
+      }
+    }
+    out
+  }
+
+  function JournalFreeze(ej: EphemeralJournal, startLsn: LSN, endLsn: LSN) : PersistentJournal
+    // requires EWF(ej);
+    // requires JournalCanFreeze(ej, startLsn, endLsn)
+    // ensures PWF(out)
+    // ensures IPJ(out) == IEJ(ej).DiscardOld(startLsn).DiscardRecent(endLsn)
+  {
+    if startLsn==endLsn
+    then
+      var out := TruncatedJournal(startLsn, None);
+      assert PWF(out);
+      assert IPJ(out) == IEJ(ej).DiscardOld(startLsn).DiscardRecent(endLsn);
+      out
+    else
+      var tj := ej.truncatedJournal;
+      var receiptLines := BuildReceipt(tj.boundaryLSN, tj.freshestRec).lines;
+      var i:nat :| JournalCanFreezeAt(ej, startLsn, endLsn, i);
+      var out := TruncatedJournal(startLsn, Some(receiptLines[i].journalRec));
+      assert PWF(out);
+      assert IPJ(out) == IEJ(ej).DiscardOld(startLsn).DiscardRecent(endLsn);
+      out
+  }
+
+  // TODO(jonh): internal operation to truncate old journal garbage
+  // TODO(jonh): internal operation to marshall tail
+}
